Bite the bullet and cleanup the representation of constructors of inductives in the environment. Direct access to the contexts of indices and sort of an indutive, and constructor arguments and conclusion indices.

template-coq/theories/Environment.v
@@ -15,11 +15,11 @@ Module Type Term.
   Parameter Inline tProj : projection -> term -> term.
   Parameter Inline mkApps : term -> list term -> term.
 
-  Parameter lift : nat -> nat -> term -> term.
-  Parameter subst : list term -> nat -> term -> term.
-  Parameter closedn : nat -> term -> bool.
-  Parameter noccur_between : nat -> nat -> term -> bool.
-  Parameter subst_instance_constr : UnivSubst term.
+  Parameter Inline lift : nat -> nat -> term -> term.
+  Parameter Inline subst : list term -> nat -> term -> term.
+  Parameter Inline closedn : nat -> term -> bool.
+  Parameter Inline noccur_between : nat -> nat -> term -> bool.
+  Parameter Inline subst_instance_constr : UnivSubst term.
   
 End Term.
 
@@ -240,26 +240,44 @@ Module Environment (T : Term).
   
   (** *** Environments *)
 
+  Record constructor_body := {
+    cstr_name : ident;
+    (* The arguments and indices are typeable under the context of 
+      arities of the mutual inductive + parameters *)
+    cstr_args : context;
+    cstr_indices : list term;
+    cstr_type : term; 
+    (* Closed type: on well-formed constructors: forall params, cstr_args, I params cstr_indices *)
+    cstr_arity : nat; (* arity, w/o lets, w/o parameters *)
+  }.
+
+  Definition map_constructor_body npars arities f c :=
+    {| cstr_name := c.(cstr_name);
+       cstr_args := fold_context (fun x => f (x + npars + arities)) c.(cstr_args);
+       cstr_indices := map (f (npars + arities + #|c.(cstr_args)|)) c.(cstr_indices);
+       cstr_type := f 0 c.(cstr_type);
+       cstr_arity := c.(cstr_arity) |}.
+
   (** See [one_inductive_body] from [declarations.ml]. *)
   Record one_inductive_body := {
     ind_name : ident;
-    ind_type : term; (* Closed arity *)
+    ind_indices : context; (* Indices of the inductive types, under params *)
+    ind_sort : Universe.t; (* Sort of the inductive. *)
+    ind_type : term; (* Closed arity = forall mind_params, ind_indices, tSort ind_sort *)
     ind_kelim : allowed_eliminations; (* Allowed eliminations *)
-    ind_ctors : list (ident * term (* Under context of arities of the mutual inductive *)
-                      * nat (* arity, w/o lets, w/o parameters *));
+    ind_ctors : list constructor_body;
     ind_projs : list (ident * term); (* names and types of projections, if any.
                                       Type under context of params and inductive object *)
     ind_relevance : relevance (* relevance of the inductive definition *) }.
 
-  Definition map_one_inductive_body npars arities f (n : nat) m :=
+  Definition map_one_inductive_body npars arities f m :=
     match m with
-    | Build_one_inductive_body ind_name ind_type ind_kelim ind_ctors ind_projs ind_relevance =>
-      Build_one_inductive_body ind_name
-                               (f 0 ind_type)
-                               ind_kelim
-                               (map (on_pi2 (f arities)) ind_ctors)
-                               (map (on_snd (f (S npars))) ind_projs)
-                               ind_relevance
+    | Build_one_inductive_body ind_name ind_indices ind_sort 
+        ind_type ind_kelim ind_ctors ind_projs ind_relevance =>
+      Build_one_inductive_body
+         ind_name (fold_context (fun x => f (npars + x)) ind_indices) ind_sort
+                  (f 0 ind_type) ind_kelim (map (map_constructor_body npars arities f) ind_ctors)
+                  (map (on_snd (f (S npars))) ind_projs) ind_relevance
     end.
 
 
@@ -462,17 +480,17 @@ Module Environment (T : Term).
       let arities := arities_context ind_bodies in
       let pars := fold_context f ind_pars in
       Build_mutual_inductive_body finite ind_npars pars
-                                  (mapi (map_one_inductive_body (context_assumptions pars) (length arities) f) ind_bodies)
+                                  (map (map_one_inductive_body (context_assumptions pars) (length arities) f) ind_bodies)
                                   ind_universes ind_variance
     end.
 
-  Lemma ind_type_map f npars_ass arities n oib :
-    ind_type (map_one_inductive_body npars_ass arities f n oib) = f 0 (ind_type oib).
+  Lemma ind_type_map f npars_ass arities oib :
+    ind_type (map_one_inductive_body npars_ass arities f oib) = f 0 (ind_type oib).
   Proof. destruct oib. reflexivity. Qed.
 
-  Lemma ind_ctors_map f npars_ass arities n oib :
-    ind_ctors (map_one_inductive_body npars_ass arities f n oib) =
-    map (on_pi2 (f arities)) (ind_ctors oib).
+  Lemma ind_ctors_map f npars_ass arities oib :
+    ind_ctors (map_one_inductive_body npars_ass arities f oib) =
+    map (map_constructor_body npars_ass arities f) (ind_ctors oib).
   Proof. destruct oib; simpl; reflexivity. Qed.
 
   Lemma ind_pars_map f m :
@@ -480,8 +498,8 @@ Module Environment (T : Term).
     fold_context f (ind_params m).
   Proof. destruct m; simpl; reflexivity. Qed.
 
-  Lemma ind_projs_map f npars_ass arities n oib :
-    ind_projs (map_one_inductive_body npars_ass arities f n oib) =
+  Lemma ind_projs_map f npars_ass arities oib :
+    ind_projs (map_one_inductive_body npars_ass arities f oib) =
     map (on_snd (f (S npars_ass))) (ind_projs oib).
   Proof. destruct oib; simpl. reflexivity. Qed.
 
@@ -546,8 +564,6 @@ Module Environment (T : Term).
     rewrite nth_error_fold_context_eq.
     do 2 f_equal. lia. now rewrite fold_context_length.
   Qed.
-
-
 
 End Environment.
 
