template-coq/theories/EnvironmentTyping.v
@@ -395,25 +395,9 @@ Module DeclarationTyping (T : Term) (E : EnvironmentSig T)
       | _, _ => False
       end.
 
-    Implicit Types (mdecl : mutual_inductive_body) (idecl : one_inductive_body) (cdecl : ident * term * nat).
+    Implicit Types (mdecl : mutual_inductive_body) (idecl : one_inductive_body) (cdecl : constructor_body).
 
     Definition on_type Σ Γ T := P Σ Γ T None.
-
-    Definition cdecl_type cdecl := cdecl.1.2.
-    Definition cdecl_args cdecl := cdecl.2.
-
-    (* A constructor shape is a decomposition of a constructor's type *)
-    Record constructor_shape :=
-      { cshape_args : context;
-        (* Arguments (with lets) *)
-
-        cshape_indices : list term;
-        (* Indices of the constructor, whose length should be the real arguments
-        length of the inductive *)
-
-        cshape_sorts : list Universe.t;
-        (* The sorts of the arguments context (without lets) *)
-      }.
 
     Open Scope type_scope.
 
@@ -588,59 +572,59 @@ Module DeclarationTyping (T : Term) (E : EnvironmentSig T)
       match variance_universes univs v with
       | Some (univs, u, u') =>
         cumul_ctx_rel (Σ, univs) (subst_instance_context u (ind_arities mdecl ,,, smash_context [] (ind_params mdecl)))
-          (subst_instance_context u (expand_lets_ctx (ind_params mdecl) (smash_context [] (cshape_args cs))))
-          (subst_instance_context u' (expand_lets_ctx (ind_params mdecl) (smash_context [] (cshape_args cs)))) *
+          (subst_instance_context u (expand_lets_ctx (ind_params mdecl) (smash_context [] (cstr_args cs))))
+          (subst_instance_context u' (expand_lets_ctx (ind_params mdecl) (smash_context [] (cstr_args cs)))) *
         All2 
-          (conv (Σ, univs) (subst_instance_context u (ind_arities mdecl ,,, smash_context [] (ind_params mdecl ,,, cshape_args cs))))
-          (map (subst_instance_constr u ∘ expand_lets (ind_params mdecl ,,, cshape_args cs)) (cshape_indices cs))
-          (map (subst_instance_constr u' ∘ expand_lets (ind_params mdecl ,,, cshape_args cs)) (cshape_indices cs))
+          (conv (Σ, univs) (subst_instance_context u (ind_arities mdecl ,,, smash_context [] (ind_params mdecl ,,, cstr_args cs))))
+          (map (subst_instance_constr u ∘ expand_lets (ind_params mdecl ,,, cstr_args cs)) (cstr_indices cs))
+          (map (subst_instance_constr u' ∘ expand_lets (ind_params mdecl ,,, cstr_args cs)) (cstr_indices cs))
       | None => False (* Monomorphic inductives have no variance attached *)
       end.
 
-    Record on_constructor Σ mdecl i idecl ind_indices cdecl (cshape : constructor_shape) := {
+    Record on_constructor Σ mdecl i idecl ind_indices cdecl cunivs := {
       (* cdecl.1 fresh ?? *)
-      cstr_args_length : context_assumptions (cshape_args cshape) = cdecl_args cdecl;
+      cstr_args_length : context_assumptions (cstr_args cdecl) = cstr_arity cdecl;
       
       (* Real (non-let) arguments bound by the constructor *)
       cstr_concl_head := tRel (#|mdecl.(ind_bodies)|
       - S i
       + #|mdecl.(ind_params)|
-      + #|cshape_args cshape|);
+      + #|cstr_args cdecl|);
       (* Conclusion head: reference to the current inductive in the block *)
 
-      cstr_eq : cdecl_type cdecl =
+      cstr_eq : cstr_type cdecl =
        it_mkProd_or_LetIn mdecl.(ind_params)
-                          (it_mkProd_or_LetIn (cshape_args cshape)
+                          (it_mkProd_or_LetIn (cstr_args cdecl)
                               (mkApps cstr_concl_head
-                              (to_extended_list_k mdecl.(ind_params) #|cshape_args cshape|
-                                ++ cshape_indices cshape)));
+                              (to_extended_list_k mdecl.(ind_params) #|cstr_args cdecl|
+                                ++ cstr_indices cdecl)));
       (* The type of the constructor canonically has this shape: parameters, real
         arguments ending with a reference to the inductive applied to the
         (non-lets) parameters and arguments *)
 
-      on_ctype : on_type Σ (arities_context mdecl.(ind_bodies)) (cdecl_type cdecl);
+      on_ctype : on_type Σ (arities_context mdecl.(ind_bodies)) (cstr_type cdecl);
       on_cargs :
         sorts_local_ctx Σ (arities_context mdecl.(ind_bodies) ,,, mdecl.(ind_params))
-                      cshape.(cshape_args) cshape.(cshape_sorts);
+                      cdecl.(cstr_args) cunivs;
       on_cindices : 
-        ctx_inst (fun Σ Γ t T => P Σ Γ t (Some T)) Σ (arities_context mdecl.(ind_bodies) ,,, mdecl.(ind_params) ,,, cshape.(cshape_args))
-                      cshape.(cshape_indices)
-                      (List.rev (lift_context #|cshape.(cshape_args)| 0 ind_indices));
+        ctx_inst (fun Σ Γ t T => P Σ Γ t (Some T)) Σ (arities_context mdecl.(ind_bodies) ,,, mdecl.(ind_params) ,,, cdecl.(cstr_args))
+                      cdecl.(cstr_indices)
+                      (List.rev (lift_context #|cdecl.(cstr_args)| 0 ind_indices));
 
       on_ctype_positive : (* The constructor type is positive *)
-        positive_cstr mdecl i [] (cdecl_type cdecl);
+        positive_cstr mdecl i [] (cstr_type cdecl);
 
       on_ctype_variance : (* The constructor type respect the variance annotation 
         on polymorphic universes, if any. *)
         forall v, ind_variance mdecl = Some v -> 
-        cstr_respects_variance Σ mdecl v cshape
+        cstr_respects_variance Σ mdecl v cdecl
     }.
 
-    Arguments on_ctype {Σ mdecl i idecl ind_indices cdecl cshape}.
-    Arguments on_cargs {Σ mdecl i idecl ind_indices cdecl cshape}.
-    Arguments on_cindices {Σ mdecl i idecl ind_indices cdecl cshape}.
-    Arguments cstr_args_length {Σ mdecl i idecl ind_indices cdecl cshape}.
-    Arguments cstr_eq {Σ mdecl i idecl ind_indices cdecl cshape}.
+    Arguments on_ctype {Σ mdecl i idecl ind_indices cdecl cunivs}.
+    Arguments on_cargs {Σ mdecl i idecl ind_indices cdecl cunivs}.
+    Arguments on_cindices {Σ mdecl i idecl ind_indices cdecl cunivs}.
+    Arguments cstr_args_length {Σ mdecl i idecl ind_indices cdecl cunivs}.
+    Arguments cstr_eq {Σ mdecl i idecl ind_indices cdecl cunivs}.
 
     Definition on_constructors Σ mdecl i idecl ind_indices :=
       All2 (on_constructor Σ mdecl i idecl ind_indices).
@@ -668,9 +652,9 @@ Module DeclarationTyping (T : Term) (E : EnvironmentSig T)
     Lemma projs_length ind npars k : #|projs ind npars k| = k.
     Proof. induction k; simpl; auto. Qed.
 
-    Definition on_projection mdecl mind i cshape (k : nat) (p : ident * term) :=
-      let Γ := smash_context [] (cshape.(cshape_args) ++ mdecl.(ind_params)) in
-      match nth_error Γ (context_assumptions cshape.(cshape_args) - S k) with
+    Definition on_projection mdecl mind i cdecl (k : nat) (p : ident * term) :=
+      let Γ := smash_context [] (cdecl.(cstr_args) ++ mdecl.(ind_params)) in
+      match nth_error Γ (context_assumptions cdecl.(cstr_args) - S k) with
       | None => False
       | Some decl => 
         let u := abstract_instance mdecl.(ind_universes) in
@@ -685,7 +669,7 @@ Module DeclarationTyping (T : Term) (E : EnvironmentSig T)
                 (lift 1 k (decl_type decl))))
       end.
 
-    Record on_projections mdecl mind i idecl (ind_indices : context) cshape :=
+    Record on_projections mdecl mind i idecl (ind_indices : context) cdecl :=
       { on_projs_record : #|idecl.(ind_ctors)| = 1;
         (** The inductive must be a record *)
 
@@ -695,81 +679,82 @@ Module DeclarationTyping (T : Term) (E : EnvironmentSig T)
         on_projs_elim : idecl.(ind_kelim) = IntoAny;
         (** This ensures that all projections are definable *)
 
-        on_projs_all : #|idecl.(ind_projs)| = context_assumptions (cshape_args cshape);
+        on_projs_all : #|idecl.(ind_projs)| = context_assumptions (cstr_args cdecl);
         (** There are as many projections as (non-let) constructor arguments *)
 
-        on_projs : Alli (on_projection mdecl mind i cshape) 0 idecl.(ind_projs) }.
+        on_projs : Alli (on_projection mdecl mind i cdecl) 0 idecl.(ind_projs) }.
 
-    Definition check_constructors_smaller φ cshapes ind_sort :=
-      Forall (fun cs => 
-        Forall (fun argsort => leq_universe φ argsort ind_sort) cs.(cshape_sorts)) cshapes.
+    Definition check_constructors_smaller φ cunivss ind_sort :=
+      Forall (fun cunivs => 
+        Forall (fun argsort => leq_universe φ argsort ind_sort) cunivs) cunivss.
 
     (** This ensures that all sorts in kelim are lower
         or equal to the top elimination sort, if set.
         For inductives in Type we do not check [kelim] currently. *)
-    
-    Definition elim_sort_prop_ind (ind_ctors_sort : list constructor_shape) :=
+
+    Definition constructor_univs := list Universe.t.
+    (* The sorts of the arguments context (without lets) *)
+
+    Definition elim_sort_prop_ind (ind_ctors_sort : list constructor_univs) :=
       match ind_ctors_sort with
       | [] => (* Empty inductive proposition: *) IntoAny
       | [ s ] =>
-        if forallb Universes.is_propositional (cshape_sorts s) then
+        if forallb Universes.is_propositional s then
           IntoAny (* Singleton elimination *)
         else
           IntoPropSProp (* Squashed: some arguments are higher than Prop, restrict to Prop *)
       | _ => (* Squashed: at least 2 constructors *) IntoPropSProp
       end.
       
-    Fixpoint elim_sort_sprop_ind (ind_ctors_sort : list constructor_shape) :=
+    Fixpoint elim_sort_sprop_ind (ind_ctors_sort : list constructor_univs) :=
       match ind_ctors_sort with
       | [] => (* Empty inductive strict proposition: *) IntoAny
       | _ => (* All other inductives in SProp are squashed *) IntoSProp
       end.
 
     Definition check_ind_sorts (Σ : global_env_ext)
-              params kelim ind_indices cshapes ind_sort : Type :=
+              params kelim ind_indices cdecls ind_sort : Type :=
       if Universe.is_prop ind_sort then
         (** The inductive is declared in the impredicative sort Prop *)
         (** No universe-checking to do: any size of constructor argument is allowed,
             however elimination restrictions apply. *)
-        allowed_eliminations_subset kelim (elim_sort_prop_ind cshapes)
+        allowed_eliminations_subset kelim (elim_sort_prop_ind cdecls)
       else if Universe.is_sprop ind_sort then
         (** The inductive is declared in the impredicative sort SProp *)
         (** No universe-checking to do: any size of constructor argument is allowed,
             however elimination restrictions apply. *)
-        allowed_eliminations_subset kelim (elim_sort_sprop_ind cshapes)
+        allowed_eliminations_subset kelim (elim_sort_sprop_ind cdecls)
       else
         (** The inductive is predicative: check that all constructors arguments are
             smaller than the declared universe. *)
-        check_constructors_smaller Σ cshapes ind_sort
+        check_constructors_smaller Σ cdecls ind_sort
         × if indices_matter then
             type_local_ctx Σ params ind_indices ind_sort
           else True.
-
+      
     Record on_ind_body Σ mind mdecl i idecl :=
       { (** The type of the inductive must be an arity, sharing the same params
             as the rest of the block, and maybe having a context of indices. *)
-        ind_indices : context;
-        ind_sort : Universe.t;
         ind_arity_eq : idecl.(ind_type)
                       = it_mkProd_or_LetIn mdecl.(ind_params)
-                                (it_mkProd_or_LetIn ind_indices (tSort ind_sort));
+                                (it_mkProd_or_LetIn idecl.(ind_indices) (tSort idecl.(ind_sort)));
 
         (** It must be well-typed in the empty context. *)
         onArity : on_type Σ [] idecl.(ind_type);
 
-        (** The decompose shapes of each constructor *)
-        ind_cshapes : list constructor_shape;
+        (** The sorts of the arguments contexts of each constructor *)
+        ind_cunivs : list constructor_univs;
 
         (** Constructors are well-typed *)
         onConstructors :
-          on_constructors Σ mdecl i idecl ind_indices idecl.(ind_ctors) ind_cshapes;
+          on_constructors Σ mdecl i idecl idecl.(ind_indices) idecl.(ind_ctors) ind_cunivs;
 
         (** Projections, if any, are well-typed *)
         onProjections :
           idecl.(ind_projs) <> [] ->
-          match ind_cshapes return Type with
+          match idecl.(ind_ctors) return Type with
           | [ o ] =>
-            on_projections mdecl mind i idecl ind_indices o
+            on_projections mdecl mind i idecl idecl.(ind_indices) o
           | _ => False
           end;
 
@@ -778,12 +763,12 @@ Module DeclarationTyping (T : Term) (E : EnvironmentSig T)
             are declared in [on_constructors]. *)
         ind_sorts :
           check_ind_sorts Σ mdecl.(ind_params) idecl.(ind_kelim)
-                          ind_indices ind_cshapes ind_sort;
+                          idecl.(ind_indices) ind_cunivs idecl.(ind_sort);
 
         onIndices : 
           (* The inductive type respect the variance annotation  on polymorphic universes, if any. *)
           forall v, ind_variance mdecl = Some v -> 
-          ind_respects_variance Σ mdecl v ind_indices
+          ind_respects_variance Σ mdecl v idecl.(ind_indices)
       }.
 
     Definition on_variance univs (variances : option (list Variance.t)) :=
@@ -869,18 +854,16 @@ Module DeclarationTyping (T : Term) (E : EnvironmentSig T)
 
   End GlobalMaps.
 
-  Arguments cstr_args_length {_ P Σ mdecl i idecl ind_indices cdecl cshape}.
-  Arguments cstr_eq {_ P Σ mdecl i idecl ind_indices cdecl cshape}.
-  Arguments on_ctype {_ P Σ mdecl i idecl ind_indices cdecl cshape}.
-  Arguments on_cargs {_ P Σ mdecl i idecl ind_indices cdecl cshape}.
-  Arguments on_cindices {_ P Σ mdecl i idecl ind_indices cdecl cshape}.
-  Arguments on_ctype_positive {_ P Σ mdecl i idecl ind_indices cdecl cshape}.
-  Arguments on_ctype_variance {_ P Σ mdecl i idecl ind_indices cdecl cshape}.
+  Arguments cstr_args_length {_ P Σ mdecl i idecl ind_indices cdecl cunivs}.
+  Arguments cstr_eq {_ P Σ mdecl i idecl ind_indices cdecl cunivs}.
+  Arguments on_ctype {_ P Σ mdecl i idecl ind_indices cdecl cunivs}.
+  Arguments on_cargs {_ P Σ mdecl i idecl ind_indices cdecl cunivs}.
+  Arguments on_cindices {_ P Σ mdecl i idecl ind_indices cdecl cunivs}.
+  Arguments on_ctype_positive {_ P Σ mdecl i idecl ind_indices cdecl cunivs}.
+  Arguments on_ctype_variance {_ P Σ mdecl i idecl ind_indices cdecl cunivs}.
 
-  Arguments ind_indices {_ P Σ mind mdecl i idecl}.
-  Arguments ind_sort {_ P Σ mind mdecl i idecl}.
   Arguments ind_arity_eq {_ P Σ mind mdecl i idecl}.
-  Arguments ind_cshapes {_ P Σ mind mdecl i idecl}.
+  Arguments ind_cunivs {_ P Σ mind mdecl i idecl}.
   Arguments onArity {_ P Σ mind mdecl i idecl}.
   Arguments onConstructors {_ P Σ mind mdecl i idecl}.
   Arguments onProjections {_ P Σ mind mdecl i idecl}.
